overhaul of the types.

Verse/Types.v
@@ -10,8 +10,14 @@ Require BinNums.
 The assembly language supported by verse is typed. We have the
 multi-word, array types and the type of sequences.
 
-** Words and vectors.
+** Words.
 
+The type [word n] denotes words of [2^n] bytes. A [vector m n] denotes
+a vector of [2^m] words of size [2^n] bytes each.
+
+** Vectors.
+
+The type [vector n w] denotes
 The type [word n] denotes words of [2^n] bytes. A [vector m n] denotes
 a vector of [2^m] words of size [2^n] bytes each.
 
@@ -35,47 +41,138 @@ verse does not allow nested streams.
 
 *)
 
-Inductive kind :=
-| bounded   : nat -> kind
-| unbounded : kind
+Inductive value := Scalar | Vector.
+Inductive bound :=
+| Value : value -> bound
+| Array
 .
 
-Definition value := bounded 0.
+Inductive kind :=
+| Bounded   : bound -> kind
+| Unbounded : kind
+.
+
+Definition valueK  (v : value) := Bounded (Value v).
+Definition scalarK := valueK Scalar.
+Definition vectorK := valueK Vector.
+Definition arrayK  := Bounded Array.
+
+
 (** The abstract syntax is specified in this module *)
 Inductive type       : kind -> Type :=
-| vector             : nat -> nat  -> type value
-| array    (n : nat) : endian
-                       -> type value
-                       -> type (bounded n)
-| sequence {n : nat} : type (bounded n)      -> type unbounded
+| word               : nat -> type (Bounded (Value Scalar))
+| vector             : nat
+                     -> type (Bounded (Value Scalar))
+                     -> type (Bounded (Value Vector))
+| array (n : nat){v : value} : endian
+                             -> type (Bounded (Value v))
+                             -> type (Bounded Array)
+| sequence {b : bound} : type (Bounded b) -> type Unbounded
 with endian : Type := bigE  | littleE | hostE.
 
-(** Some common types **)
-Definition Word   := vector 0.
-Definition Byte   := Word 0. (** 2^0 = 1 byte *)
-Definition Word8  := Word 0. (** 2^0 = 1 byte *)
-Definition Word16 := Word 1. (** 2^1 = 2 byte *)
-Definition Word32 := Word 2. (** 2^2 = 4 byte *)
-Definition Word64 := Word 3. (** 2^3 = 8 byte *)
+(** Word types that are commonly found in machines *)
+
+Definition Byte   := word 0. (** 2^0 = 1 byte *)
+Definition Word8  := word 0. (** 2^0 = 1 byte *)
+Definition Word16 := word 1. (** 2^1 = 2 byte *)
+Definition Word32 := word 2. (** 2^2 = 4 byte *)
+Definition Word64 := word 3. (** 2^3 = 8 byte *)
+
+(* ** Common vector types
+
+We have vector types of 128-bits and 256 bits given by
+[Vector128_*] and [Vector256_*].
+
+ *)
+
+Definition Vector128_64   := vector 1 Word64.
+Definition Vector128_32   := vector 2 Word32.
+Definition Vector128_16   := vector 3 Word16.
+Definition Vector128_8    := vector 4 Word8.
+Definition Vector128Bytes := vector 4 Byte.
+
+Definition Vector256_64   := vector 2 Word64.
+Definition Vector256_32   := vector 3 Word32.
+Definition Vector256_16   := vector 4 Word16.
+Definition Vector256_8    := vector 5 Word8.
+Definition Vector256Bytes := vector 5 Byte.
+
+(**
+
+This module proves the correctness of the vector types defined
+
+*)
+Module VectorCorrectness.
+
+  (**
+
+      When you make a vector of 128-bits of word type n, you need to
+      ensure that the total bits are of exactly 128 bits long. If you
+      use vector k n, then this means that [2^k * 2^n = 128] or in
+      other words [k + n = 4]. We prove these theorems here.
+
+   *)
+
+  Definition WFVector128 (v : type vectorK) : Prop
+    := match v with
+         | vector n (word m) => n + m = 4
+         | _                 => False
+       end.
+  Definition WFVector256 (v : type vectorK) : Prop
+    := match v with
+         | vector n (word m) => n + m = 5
+         | _                 => False
+       end.
+
+  Theorem v128_64WF : WFVector128 (Vector128_64).
+  Proof.
+    crush_inequalities.
+  Qed.
+
+  Theorem v128_32WF : WFVector128 (Vector128_32).
+  Proof.
+    crush_inequalities.
+  Qed.
+
+  Theorem v128_16WF : WFVector128 (Vector128_16).
+  Proof.
+    crush_inequalities.
+  Qed.
+
+  Theorem v128_8WF : WFVector128 (Vector128_8).
+  Proof.
+    crush_inequalities.
+  Qed.
+
+  Theorem v128_ByteWF : WFVector128 (Vector128Bytes).
+  Proof.
+    crush_inequalities.
+  Qed.
 
 
-(** A constant of a given type *)
-Inductive constant  : type value -> Type :=
-| w {n : nat}   : Vector.t nat  (2 ^ n) -> constant (Word n)
-| v {m n : nat} : Vector.t (constant (Word n)) (2 ^ m)
-                  -> constant (vector m n).
 
-Definition valuetype := type (bounded 0).
+  Theorem v256_64WF : WFVector256 (Vector256_64).
+  Proof.
+    crush_inequalities.
+  Qed.
 
-Ltac makeArray n e t :=
-  match n with
-    | 0 => fail 1 "array of length 0 defined"
-    | _ => exact (array n e t)
-  end.
+  Theorem v256_32WF : WFVector256 (Vector256_32).
+  Proof.
+    crush_inequalities.
+  Qed.
 
+  Theorem v256_16WF : WFVector256 (Vector256_16).
+  Proof.
+    crush_inequalities.
+  Qed.
 
-Definition bigEndian (n : nat)(t : type (bounded 0))
-  := array n bigE t.
+  Theorem v256_8WF : WFVector256 (Vector256_8).
+  Proof.
+    crush_inequalities.
+  Qed.
 
-Definition littleEndian (n : nat)(t : type (bounded 0))
-  := array n littleE t.
+  Theorem v256_ByteWF : WFVector256 (Vector256Bytes).
+  Proof.
+    crush_inequalities.
+  Qed.
+End VectorCorrectness.
